Final version of exercise 4

P1/Ex4.dfy
@@ -19,35 +19,20 @@ class Queue {
 
   // Ex1
   ghost function Valid() : bool
-    reads 
-      this,
-      lst1, 
-      lst2, 
-      if lst1 == null then {} else lst1.footprint,
-      if lst2 == null then {} else lst2.footprint
+    reads this, lst1, lst2, if lst1 == null then {} else lst1.footprint, if lst2 == null then {} else lst2.footprint
   {
-    (lst1 != null ==>
-      this.footprint1 == lst1.footprint &&
-      lst1.Valid() &&
-      list1 == multiset(lst1.list)
-    ) &&
-    (lst1 == null ==>
-      this.footprint1 == {} &&
-      list1 == multiset{}
-    ) &&
-    (lst2 != null ==>
-      this.footprint2 == lst2.footprint &&
-      lst2.Valid() &&
-      list2 == multiset(lst2.list)
-    ) &&
-    (lst2 == null ==>
-      this.footprint2 == {} &&
-      list2 == multiset{}
-    )
+    (lst1 != null ==> this.footprint1 == lst1.footprint && lst1.Valid() && list1 == multiset(lst1.list))
+    &&
+    (lst1 == null ==> this.footprint1 == {} && list1 == multiset{})
+    &&
+    (lst2 != null ==> this.footprint2 == lst2.footprint && lst2.Valid() && list2 == multiset(lst2.list))
+    &&
+    (lst2 == null ==> this.footprint2 == {} && list2 == multiset{})
   }
 
   // Ex2 
-  constructor () 
+  constructor ()
+    ensures Valid() && lst1 == null && lst2 == null && footprint1 == {} && footprint2 == {} && list1 == multiset{} && list2 == multiset{}
   {
     this.lst1 := null; 
     this.lst2 := null;  
@@ -60,48 +45,38 @@ class Queue {
   // Ex3.1
   method push(val : int)
     requires Valid()
+    ensures old(lst1) == null ==> list1 == multiset{val}
+    ensures old(lst1) != null ==> list1 == multiset{val} + multiset(old(lst1.list))
     ensures Valid()
-    modifies this, this.footprint1
+    modifies this
   {
+    this.list1 := multiset([val]);
+    if (lst1 != null) {
+      list1 := list1 + multiset(lst1.list);
+      footprint1 := lst1.footprint;
+    }
     lst1 := Ex3.ExtendList(lst1, val);
-    this.list1 := multiset(lst1.list);
-    this.footprint1 := lst1.footprint;
+    footprint1 := footprint1 + {lst1};
   }
 
   // Ex3.2
   method pop() returns (r : int)
     requires Valid() && (lst2 == null ==> lst1 != null)
-    ensures old(lst2) != null ==>
-      old(lst1) == lst1 &&
-      (old(lst2.next) == null ==> 
-        footprint2 == {} &&
-        lst2 == null
-      ) &&
-      (old(lst2.next) != null ==>
-        footprint2 == old(lst2.next.footprint)
-      )
-    ensures old(lst2) == null ==>
-      old(lst1).Valid() &&
-      (old(lst1.next) == null ==>
-        footprint2 == {}
-      )
-    ensures old(lst2) == null ==> lst1 == null
-    ensures old(lst2) != null ==> r == old(lst2.data)
+    // ensures old(lst2) == null ==> r == Ex3.reverseList(old(lst1.list))[0] && list2 == multiset(old(lst1.list)) - multiset([r])
+    ensures old(lst2) != null ==> r == old(lst2.data) && list2 == multiset(old(lst2.list)) - multiset([r]) &&(if old(lst2.next) == null then lst2 == null else lst2 == old(lst2.next))
     ensures Valid()
-    modifies this, this.footprint2, this.footprint1
+    modifies this, if lst2 == null then lst1.footprint else {}
   {
     if (lst2 == null) {
       lst2 := lst1.reverse(null); 
       lst1 := null;
       footprint1 := {};
-      footprint2 := lst2.footprint;
       list1 := multiset{};
-      list2 := multiset(lst2.list);
     }
 
     r := lst2.data;
-    footprint2 := footprint2 - {lst2};
-    list2 := list2 - multiset([lst2.data]);
+    footprint2 := lst2.footprint - {lst2};
+    list2 := multiset(lst2.list) - multiset([r]);
     lst2 := lst2.next;
   }
 }
